src/coq/Dot_Examples.v
@@ -11,27 +11,52 @@ Hint Constructors vars_ok_tp valid_label.
 Hint Constructors typing expands sub_tp sub_decl wf_tp wf_decl wfe_tp.
 Hint Unfold decls_ok decls_uniq.
 
+Tactic Notation
+  "pick" "fresh" ident(atom_name) "and" ident(atom_name')
+  "excluding" constr(L) "and" constr(L')
+  "and" "apply" constr(H)
+  :=
+    first [apply (@H L L') | eapply (@H L L')];
+      match goal with
+        | |- forall _, _ `notin` _ -> _ =>
+          let Fr := fresh "Fr" in intros atom_name Fr
+        | |- forall _, _ `notin` _ -> _ =>
+          fail 1 "because" atom_name "is already defined"
+        | _ =>
+          idtac
+      end.
+
+Tactic Notation
+  "pick" "fresh" ident(atom_name) "and" ident(atom_name')
+  "and" "apply" constr(H)
+  :=
+    let L := gather_atoms in
+    let L := beautify_fset L in
+    let L' := gather_atoms in
+    let L' := beautify_fset L' in
+    pick fresh atom_name and atom_name' excluding L and L' and apply H.
+
 Ltac crush_rules :=
   repeat (match goal with
-            | [ |- ?S |~ app (lam ?T ?B) ?V ~~> ?R ~| ?S ] => apply red_beta
-            | [ |- ?E |= (lam ?T ?B) ~: _ ] => let x := fresh "x" in pick fresh x and apply typing_abs
-            | [ |- ?E |= (new ?X ?Tc ?args) ~: _ ] => let x := fresh "x" in pick fresh x and apply typing_new
+(*          | [ |- ?S |~ app (lam ?T ?B) ?V ~~> ?R ~| ?S ] => apply red_beta*)
+(*          | [ |- ?E |= (lam ?T ?B) ~: _ ] => let x := fresh "x" in pick fresh x and apply typing_abs*)
+            | [ |- ?E |= (new ?X ?Tc ?args) ~: _ ] => let x := fresh "x" in let y := fresh "y" in pick fresh x and y and apply typing_new
             | [ |- ?E |= (fvar ?X) ~: _ ] => apply typing_var
             | [ |- wf_tp ?E (tp_rfn _ _) ] => let x:= fresh "x" in pick fresh x and apply wf_rfn
             | [ |- wf_env ((?X, ?T) :: ?R, ?S) ] => rewrite_env (([(X,T)] ++ R), S); apply wf_env_cons
-            | [ |- lc_tm (lam ?T ?B) ] => let x := fresh "x" in pick fresh x and apply lc_lam
+(*          | [ |- lc_tm (lam ?T ?B) ] => let x := fresh "x" in pick fresh x and apply lc_lam*)
             | [ |- lc_tm (new ?Tc ?A ?B) ] => let x:= fresh "x" in pick fresh x and apply lc_new
             | [ |- lc_tp (tp_rfn _ _) ] =>  let x:= fresh "x" in pick fresh x and apply lc_tp_rfn
-            | [ |- lc_args ( _ :: _ ) ] => apply lc_args_cons
+            | [ |- lc_args ( _ :: _ ) ] => apply lc_args_cons_value
             | [ |- wfe_tp _ tp_top ] => apply wfe_top
             | [ |- wfe_tp _ tp_bot ] => apply wfe_bot
-            | [ |- wfe_tp _ (tp_fun _ _) ] => apply wfe_fun
+(*          | [ |- wfe_tp _ (tp_fun _ _) ] => apply wfe_fun*)
             | [ |- _ |= _ ~<: tp_top ] => apply sub_tp_top
             | [ |- context[(?Y ^ ?X)] ] => unfold open; unfold open_rec_tm; simpl
             | [ |- context[(?Y ^^ ?X)] ] => unfold open; unfold open_rec_tm; simpl
             | [ |- context[(?Y ^ds^ ?X)] ] => unfold open_decls; simpl
             | [ |- context[(?Y ^dsl^ ?X)] ] => unfold open_decls_lst; simpl
-            | [ |- value (lam ?T ?B) ] => apply value_lam
+(*          | [ |- value (lam ?T ?B) ] => apply value_lam *)
             | [ |- context[decls_binds _ _ _] ] => let H:=fresh "H" in introv H; inversion H
             | [ |- context[lbl.binds _ _ _] ] => let H:=fresh "H" in introv H; inversion H
             | [ |- context[ctx_bind _ _ _] ] => unfold ctx_bind; simpl
@@ -56,9 +81,11 @@ Parameter Lt : label.
 Axiom Lt_type_label : type_label Lt.
 Hint Resolve Lt_type_label.
 
+(*
 Definition ex1 := app (lam tp_top 0) (lam tp_top 0).
 Example ex1_red : nil |~ ex1 ~~> (lam tp_top 0) ~| nil.
 Proof. unfold ex1. crush_rules. Qed.
+*)
 
 Definition ex2 := new tp_top nil 0.
 Example ex2_red : exists a, nil |~ ex2 ~~> 0 ^^ (ref a) ~| ((a ~ (tp_top, nil)) ++ nil).
@@ -72,23 +99,30 @@ Proof.
   unfold ex3. pick fresh a. exists a. eexists. apply red_new; crush_rules.
 Qed.
 
+(*
 Definition ex4 := new (tp_rfn tp_top [(l, decl_tm tp_top)]) [(l, lam tp_top 0)] (sel 0 l).
 Example ex4_red : exists a, exists store', nil |~ ex4 ~~> (sel 0 l) ^^ (ref a) ~| store'.
 Proof.
   unfold ex4. pick fresh a. exists a. eexists. apply red_new; crush_rules.
 Qed.
+*)
 
+(*
 Example ex_id_typ : (nil,nil) |= (lam tp_top 0) ~: (tp_fun tp_top tp_top).
 Proof. crush_rules. Qed.
+*)
 
+(*
 Example ex1_typ : (nil,nil) |= ex1 ~: tp_top.
 Proof.
   unfold ex1. apply typing_app with (S:=tp_top) (T':=tp_fun tp_top tp_top); crush_rules.
 Qed.
+*)
 
 Example ex2_typ : (nil,nil) |= ex2 ~: tp_top.
 Proof. unfold ex2. crush_rules. Qed.
 
+(*
 Example cast_typ : (nil,nil) |= (lam tp_bot (app (lam tp_top 0) (lam (tp_sel 0 Lt) 0))) ~: tp_fun tp_bot tp_top.
 Proof.
   crush_rules.
@@ -116,5 +150,5 @@ Proof.
   apply wfe_sel_bot with (L:=empty) (x:=x); assumption.
   apply wfe_sel_bot with (L:=empty) (x:=x); assumption.
 Qed.
-
+*)
 End Ex.
